the para_beta lemma was proved, along with the other bunch of lemmas

Lambda/Confluence.lean
@@ -39,6 +39,45 @@ lemma para_shift_conservation {i j : Nat} {N N' : Lambda} : N →βp N' → (↑
         rw [← shift_shift_swap _ (Nat.zero_le i), ← beta]
         apply BetaP.subst <;> aesop
 
+lemma para_shift_shifted {d c} {N₁ N₂ : Lambda} :
+    N₁ →βp N₂ → Shifted d c N₁ → Shifted d c N₂ := by
+    intro h₁ h₂
+    induction h₁ generalizing c d with
+    | var n => assumption
+    | app => cases h₂; apply Shifted.sapp <;> aesop
+    | abs => cases h₂; apply Shifted.sabs; aesop
+    | subst M₁ M₂ L₁ L₂ hm hl ihm ihl =>
+        simp [beta]; cases h₂; rename_i h1 h2; cases h1
+        nth_rw 2 [Eq.symm (Nat.zero_add 1)]
+        rw [Eq.symm (Nat.zero_add c)]
+        apply shifted_subst <;> (first | apply ihm | apply ihl)
+        rw [Nat.zero_add, Nat.add_comm]
+        all_goals assumption
+
+lemma para_unshift_conservation {i j : Nat} {N N' : Lambda} :
+    Shifted j i N → N →βp N' → (↓) i j N →βp (↓) i j N' := by
+    intro h₁ h₂
+    induction h₂ generalizing i j with
+    | var => rfl
+    | abs => simp; cases h₁; aesop
+    | app => simp; cases h₁; constructor <;> aesop
+    | subst M₁ M₂ N₁ N₂ hm hn ihm ihn =>
+        simp [beta]; cases h₁; rename_i h1 h2; cases h1; rename_i h1
+        have hsn := para_shift_shifted hn h2
+        have hsm := para_shift_shifted hm h1
+        rw [unshift_unshift_swap (by omega) (by aesop) ?shifted]
+        case shifted =>
+            rw [Eq.symm (Nat.zero_add i)]
+            nth_rw 2 [Eq.symm (Nat.zero_add 1)]
+            apply shifted_subst <;> (try assumption)
+            rw [Nat.zero_add, Nat.add_comm]; assumption
+        rw [unshift_subst_swap2 (by omega) hsm ?shifted]
+        case shifted =>
+            rw [Nat.add_comm]; apply shift_shifted' <;> aesop
+
+        rw [← unshift_shift_swap (by omega) hsn, ← beta]
+        apply BetaP.subst <;> aesop
+
 lemma para_subst' {n} {M N N' : Lambda} : N →βp N' → M[n := N] →βp M[n := N'] := by
     intros
     induction M generalizing n N N' with
@@ -63,3 +102,41 @@ lemma para_subst {n} {M N M' N' : Lambda} :
         apply BetaP.subst
         apply ihm; apply para_shift_conservation; assumption
         all_goals aesop
+
+lemma para_beta {M N M' N' : Lambda} :
+    M →βp M' → N →βp N' → M.beta N →βp M'.beta N' := by
+    intro hm hn; simp [beta]
+    apply para_unshift_conservation
+    . exact shifted_subst' 0 M N
+    . apply (para_subst hm); exact para_shift_conservation hn
+
+lemma abs_para_abs {M N : Lambda} (h : λ M →βp N) : ∃ M', N = λ M' ∧ M →βp M' := by cases h; case abs => aesop
+
+lemma app_para_cases {M N L : Lambda} (h : M.app N →βp L) :
+    (∃ M' N', L = M'.app N' ∧ M →βp M' ∧ N →βp N') ∨
+    (∃ P P' N', M = λ P ∧ L = P'.beta N' ∧ N →βp N' ∧ P →βp P') := by
+    cases h
+    case app M' N' _ _ => left; use M', N'
+    case subst P M' N' _ _ => right; use P, M', N'
+
+def Diamond (R : α → α → Prop) := ∀ a b c, R a b → R a c → ∃ d, R b d ∧ R c d
+
+theorem para_diamond : Diamond BetaP := by
+    unfold Diamond; intro M M₁ M₂ h1 h2
+    induction h1 generalizing M₂ with
+    | var => simp at h2; simp_all
+    | abs N₁ N₂ h ih =>
+        obtain ⟨N₃, _, N₁reN₃⟩ := abs_para_abs h2
+        obtain ⟨N₄, _, _⟩ := ih N₃ N₁reN₃
+        use λ N₄; aesop
+    | app N₁ N₂ P₁ P₂ hn₁₂ hp₁₂ ihn ihp =>
+
+        rcases app_para_cases h2 with ⟨N₃, P₃, M₂eq, N₁reN₃, P₁reP₃⟩
+            | ⟨L₁, L₂, P₃, N₁eq, M₂eq, P₁reP₂, L₁reL₂⟩
+        . obtain ⟨N₄, _, _⟩ := ihn N₃ N₁reN₃
+          obtain ⟨P₄, _, _⟩ := ihp P₃ P₁reP₃
+          rw [M₂eq]
+          use N₄.app P₄; constructor <;> apply BetaP.app <;> aesop
+        .
+            sorry
+    | subst => sorry
